Phi_System/IDE_CP_Applications1.thy
@@ -937,6 +937,20 @@ lemma [\<phi>reason 1200]:
   unfolding Action_Tag_def Transformation_def
   by (cases x; simp; blast)
 
+paragraph \<open>Special Forms\<close>
+
+lemma [\<phi>reason 1000]:
+  \<open> 1 \<t>\<r>\<a>\<n>\<s>\<f>\<o>\<r>\<m>\<s> (y::'b::one) \<Ztypecolon> Itself \<s>\<u>\<b>\<j> y. y = 1 @action to (Itself :: ('b, 'b) \<phi>) \<close>
+  unfolding Action_Tag_def Transformation_def Identity_Element\<^sub>E_def
+  by simp
+
+lemma [\<phi>reason 1000]:
+  \<open> (\<c>\<o>\<n>\<d>\<i>\<t>\<i>\<o>\<n> C \<Longrightarrow> x \<Ztypecolon> A \<t>\<r>\<a>\<n>\<s>\<f>\<o>\<r>\<m>\<s> (y :: 'a) \<Ztypecolon> Itself \<s>\<u>\<b>\<j> y. ra y @action to (Itself :: ('a,'a) \<phi>))
+\<Longrightarrow> (\<c>\<o>\<n>\<d>\<i>\<t>\<i>\<o>\<n> \<not> C \<Longrightarrow> x \<Ztypecolon> B \<t>\<r>\<a>\<n>\<s>\<f>\<o>\<r>\<m>\<s> y \<Ztypecolon> Itself \<s>\<u>\<b>\<j> y. rb y @action to (Itself :: ('a,'a) \<phi>))
+\<Longrightarrow> x \<Ztypecolon> If C A B \<t>\<r>\<a>\<n>\<s>\<f>\<o>\<r>\<m>\<s> y \<Ztypecolon> Itself \<s>\<u>\<b>\<j> y. (if C then ra y else rb y) @action to (Itself :: ('a,'a) \<phi>)\<close>
+  unfolding Action_Tag_def Transformation_def Premise_def
+  by simp
+
 
 
 subsubsection \<open>The \<open>to\<close> application\<close>
