Phi_System/IDE_CP_Reasoning2.thy
@@ -210,11 +210,10 @@ Priority Convention:
 \<^item> 3200: Very Safe Normalization
 \<^item> 3150: Assigning Zeros
 \<^item> 3000: Normalization
-\<^item> 2800: Disjunction in source part; Default normalization in source part
+\<^item> 2800: Disjunction in source part
         Conjunction in target part
         Fix existentially quantified variables in source part
-\<^item> 2600: Default normalization in target part (*what is this? =.=*)
-\<^item> 2550: Top
+\<^item> 2600: Usual reasonings
 \<^item> 2100: Padding void holes after the last item. Rules capturing the whole items including
         the last item in the \<open>\<^emph>\<close>-sequence should have priority higher than this.
 \<^item> 2000: Step-by-step searching
@@ -807,88 +806,130 @@ declare [[\<phi>reason !12 NToA_disj_target_A' NToA_disj_target_B'
 
 hide_fact NToA_disj_target_A' NToA_disj_target_B'
 
-subsubsection \<open>Conditional Branch in Source\<close>
+subsubsection \<open>Conditional Branch\<close>
 
 text \<open>The condition should be regarded as an output, and the reasoning process assigns which
 the branch that it chooses to the output condition variable.\<close>
 
-lemma NToA_cond_source_A:
+paragraph \<open>Normalization\<close>
+
+lemma [\<phi>reason 2600]:
+  \<open> If C (x \<Ztypecolon> A) (x \<Ztypecolon> B) \<t>\<r>\<a>\<n>\<s>\<f>\<o>\<r>\<m>\<s> Y \<w>\<i>\<t>\<h> P
+\<Longrightarrow> x \<Ztypecolon> If C A B \<t>\<r>\<a>\<n>\<s>\<f>\<o>\<r>\<m>\<s> Y \<w>\<i>\<t>\<h> P\<close>
+  by (cases C; simp)
+
+lemma [\<phi>reason 2600]:
+  \<open> X \<t>\<r>\<a>\<n>\<s>\<f>\<o>\<r>\<m>\<s> If C (x \<Ztypecolon> A) (x \<Ztypecolon> B) \<w>\<i>\<t>\<h> P
+\<Longrightarrow> X \<t>\<r>\<a>\<n>\<s>\<f>\<o>\<r>\<m>\<s> x \<Ztypecolon> If C A B \<w>\<i>\<t>\<h> P\<close>
+  by (cases C; simp)
+
+
+paragraph \<open>In Source\<close>
+
+lemma NToA_cond_source_A[\<phi>reason 2601]:
   \<open> A \<t>\<r>\<a>\<n>\<s>\<f>\<o>\<r>\<m>\<s> X \<w>\<i>\<t>\<h> P
 \<Longrightarrow> (if True then A else B) \<t>\<r>\<a>\<n>\<s>\<f>\<o>\<r>\<m>\<s> X \<w>\<i>\<t>\<h> P\<close>
   unfolding Action_Tag_def
   by (simp add: Transformation_def distrib_left)
 
-lemma NToA_cond_source_B:
+lemma NToA_cond_source_B[\<phi>reason 2601]:
   \<open> B \<t>\<r>\<a>\<n>\<s>\<f>\<o>\<r>\<m>\<s> X \<w>\<i>\<t>\<h> P
 \<Longrightarrow> (if False then A else B) \<t>\<r>\<a>\<n>\<s>\<f>\<o>\<r>\<m>\<s> X \<w>\<i>\<t>\<h> P\<close>
   unfolding Action_Tag_def
   by (simp add: Transformation_def distrib_left)
 
-declare [[\<phi>reason 2600 NToA_cond_source_A NToA_cond_source_B
-        for \<open>(if ?condition then ?A else ?B) \<t>\<r>\<a>\<n>\<s>\<f>\<o>\<r>\<m>\<s> ?X \<w>\<i>\<t>\<h> ?P\<close>]]
+declare [[\<phi>reason !12 NToA_cond_source_A NToA_cond_source_B
+        for \<open>(if ?var_condition then ?A else ?B) \<t>\<r>\<a>\<n>\<s>\<f>\<o>\<r>\<m>\<s> ?X \<w>\<i>\<t>\<h> ?P\<close>]]
 
 hide_fact NToA_cond_source_A NToA_cond_source_B
 
-lemma NToA_cond_source_A':
+lemma [\<phi>reason 2600 except \<open>(if ?var then _ else _) \<t>\<r>\<a>\<n>\<s>\<f>\<o>\<r>\<m>\<s> _ \<w>\<i>\<t>\<h> _\<close>]:
+  \<open> (\<c>\<o>\<n>\<d>\<i>\<t>\<i>\<o>\<n> C \<Longrightarrow> (\<c>\<o>\<n>\<d>\<i>\<t>\<i>\<o>\<n> False) \<or>\<^sub>c\<^sub>u\<^sub>t (A \<t>\<r>\<a>\<n>\<s>\<f>\<o>\<r>\<m>\<s> X \<w>\<i>\<t>\<h> P))
+\<Longrightarrow> (\<c>\<o>\<n>\<d>\<i>\<t>\<i>\<o>\<n> \<not> C \<Longrightarrow> (\<c>\<o>\<n>\<d>\<i>\<t>\<i>\<o>\<n> False) \<or>\<^sub>c\<^sub>u\<^sub>t (B \<t>\<r>\<a>\<n>\<s>\<f>\<o>\<r>\<m>\<s> X \<w>\<i>\<t>\<h> P))
+\<Longrightarrow> (if C then A else B) \<t>\<r>\<a>\<n>\<s>\<f>\<o>\<r>\<m>\<s> X \<w>\<i>\<t>\<h> P \<close>
+  by (cases C; simp add: Premise_def)
+
+
+lemma NToA_cond_source_A'[\<phi>reason 2601]:
   \<open> R * A \<t>\<r>\<a>\<n>\<s>\<f>\<o>\<r>\<m>\<s> X \<w>\<i>\<t>\<h> P
 \<Longrightarrow> R * (if True then A else B) \<t>\<r>\<a>\<n>\<s>\<f>\<o>\<r>\<m>\<s> X \<w>\<i>\<t>\<h> P\<close>
   unfolding Action_Tag_def
   by (simp add: Transformation_def distrib_left)
 
-lemma NToA_cond_source_B':
+lemma NToA_cond_source_B'[\<phi>reason 2601]:
   \<open> R * B \<t>\<r>\<a>\<n>\<s>\<f>\<o>\<r>\<m>\<s> X \<w>\<i>\<t>\<h> P
 \<Longrightarrow> R * (if False then A else B) \<t>\<r>\<a>\<n>\<s>\<f>\<o>\<r>\<m>\<s> X \<w>\<i>\<t>\<h> P\<close>
   unfolding Action_Tag_def
   by (simp add: Transformation_def distrib_left)
 
-declare [[\<phi>reason 2600 NToA_cond_source_A' NToA_cond_source_B'
-        for \<open>?R * (if ?condition then ?A else ?B) \<t>\<r>\<a>\<n>\<s>\<f>\<o>\<r>\<m>\<s> ?X \<w>\<i>\<t>\<h> ?P\<close>]]
+declare [[\<phi>reason !12 NToA_cond_source_A' NToA_cond_source_B'
+        for \<open>?R * (if ?var_condition then ?A else ?B) \<t>\<r>\<a>\<n>\<s>\<f>\<o>\<r>\<m>\<s> ?X \<w>\<i>\<t>\<h> ?P\<close>]]
 
 hide_fact NToA_cond_source_A' NToA_cond_source_B'
 
+lemma [\<phi>reason 2600 except \<open>_ * (if ?var then _ else _) \<t>\<r>\<a>\<n>\<s>\<f>\<o>\<r>\<m>\<s> _ \<w>\<i>\<t>\<h> _\<close>]:
+  \<open> (\<c>\<o>\<n>\<d>\<i>\<t>\<i>\<o>\<n> C \<Longrightarrow> (\<c>\<o>\<n>\<d>\<i>\<t>\<i>\<o>\<n> False) \<or>\<^sub>c\<^sub>u\<^sub>t (R * A \<t>\<r>\<a>\<n>\<s>\<f>\<o>\<r>\<m>\<s> X \<w>\<i>\<t>\<h> P))
+\<Longrightarrow> (\<c>\<o>\<n>\<d>\<i>\<t>\<i>\<o>\<n> \<not> C \<Longrightarrow> (\<c>\<o>\<n>\<d>\<i>\<t>\<i>\<o>\<n> False) \<or>\<^sub>c\<^sub>u\<^sub>t (R * B \<t>\<r>\<a>\<n>\<s>\<f>\<o>\<r>\<m>\<s> X \<w>\<i>\<t>\<h> P))
+\<Longrightarrow> R * (if C then A else B) \<t>\<r>\<a>\<n>\<s>\<f>\<o>\<r>\<m>\<s> X \<w>\<i>\<t>\<h> P \<close>
+  by (cases C; simp add: Premise_def)
 
-subsubsection \<open>Conditional Branch in Target\<close>
 
-lemma NToA_cond_target_A:
+paragraph \<open>in Target\<close>
+
+lemma NToA_cond_target_A[\<phi>reason 2601]:
   \<open> X \<t>\<r>\<a>\<n>\<s>\<f>\<o>\<r>\<m>\<s> A \<w>\<i>\<t>\<h> P
 \<Longrightarrow> X \<t>\<r>\<a>\<n>\<s>\<f>\<o>\<r>\<m>\<s> (if True then A else B) \<w>\<i>\<t>\<h> P\<close>
   by simp
 
-lemma NToA_cond_target_B:
+lemma NToA_cond_target_B[\<phi>reason 2601]:
   \<open> X \<t>\<r>\<a>\<n>\<s>\<f>\<o>\<r>\<m>\<s> B \<w>\<i>\<t>\<h> P
 \<Longrightarrow> X \<t>\<r>\<a>\<n>\<s>\<f>\<o>\<r>\<m>\<s> (if False then A else B) \<w>\<i>\<t>\<h> P\<close>
   by simp
 
-declare [[\<phi>reason 2600 NToA_cond_target_A NToA_cond_target_B
-            for \<open>?X \<t>\<r>\<a>\<n>\<s>\<f>\<o>\<r>\<m>\<s> (if ?condition then ?A else ?B) \<w>\<i>\<t>\<h> ?P\<close> ]]
+declare [[\<phi>reason !12 NToA_cond_target_A NToA_cond_target_B
+            for \<open>?X \<t>\<r>\<a>\<n>\<s>\<f>\<o>\<r>\<m>\<s> (if ?var_condition then ?A else ?B) \<w>\<i>\<t>\<h> ?P\<close> ]]
 
 hide_fact NToA_cond_target_A NToA_cond_target_B
 
-lemma NToA_cond_target_A':
+lemma [\<phi>reason 2600 except \<open>_ \<t>\<r>\<a>\<n>\<s>\<f>\<o>\<r>\<m>\<s> (if ?var then _ else _) \<w>\<i>\<t>\<h> _\<close>]:
+  \<open> (\<c>\<o>\<n>\<d>\<i>\<t>\<i>\<o>\<n> C \<Longrightarrow> (\<c>\<o>\<n>\<d>\<i>\<t>\<i>\<o>\<n> False) \<or>\<^sub>c\<^sub>u\<^sub>t (X \<t>\<r>\<a>\<n>\<s>\<f>\<o>\<r>\<m>\<s> A \<w>\<i>\<t>\<h> P))
+\<Longrightarrow> (\<c>\<o>\<n>\<d>\<i>\<t>\<i>\<o>\<n> \<not> C \<Longrightarrow> (\<c>\<o>\<n>\<d>\<i>\<t>\<i>\<o>\<n> False) \<or>\<^sub>c\<^sub>u\<^sub>t (X \<t>\<r>\<a>\<n>\<s>\<f>\<o>\<r>\<m>\<s> B \<w>\<i>\<t>\<h> P))
+\<Longrightarrow> X \<t>\<r>\<a>\<n>\<s>\<f>\<o>\<r>\<m>\<s> (if C then A else B) \<w>\<i>\<t>\<h> P \<close>
+  by (cases C; simp add: Premise_def)
+
+
+lemma NToA_cond_target_A'[\<phi>reason 2601]:
   \<open> X \<t>\<r>\<a>\<n>\<s>\<f>\<o>\<r>\<m>\<s> R * \<blangle> A \<brangle> \<w>\<i>\<t>\<h> P
 \<Longrightarrow> X \<t>\<r>\<a>\<n>\<s>\<f>\<o>\<r>\<m>\<s> R * \<blangle> if True then A else B \<brangle> \<w>\<i>\<t>\<h> P\<close>
   by simp
 
-lemma NToA_cond_target_B':
+lemma NToA_cond_target_B'[\<phi>reason 2601]:
   \<open> X \<t>\<r>\<a>\<n>\<s>\<f>\<o>\<r>\<m>\<s> R * \<blangle> B \<brangle> \<w>\<i>\<t>\<h> P
 \<Longrightarrow> X \<t>\<r>\<a>\<n>\<s>\<f>\<o>\<r>\<m>\<s> R * \<blangle> if False then A else B \<brangle> \<w>\<i>\<t>\<h> P\<close>
   by simp
 
-declare [[\<phi>reason 2600 NToA_cond_target_B' NToA_cond_target_A'
-            for \<open>?X \<t>\<r>\<a>\<n>\<s>\<f>\<o>\<r>\<m>\<s> _ * \<blangle> if ?condition then ?A else ?B \<brangle> \<w>\<i>\<t>\<h> ?P\<close> ]]
+declare [[\<phi>reason !12 NToA_cond_target_B' NToA_cond_target_A'
+            for \<open>?X \<t>\<r>\<a>\<n>\<s>\<f>\<o>\<r>\<m>\<s> _ * \<blangle> if ?var_condition then ?A else ?B \<brangle> \<w>\<i>\<t>\<h> ?P\<close> ]]
 
 hide_fact NToA_cond_target_A' NToA_cond_target_B'
+
+lemma [\<phi>reason 2600 except \<open>_ \<t>\<r>\<a>\<n>\<s>\<f>\<o>\<r>\<m>\<s> (if ?var then _ else _) \<r>\<e>\<m>\<a>\<i>\<n>\<s> _ \<w>\<i>\<t>\<h> _\<close>]:
+  \<open> (\<c>\<o>\<n>\<d>\<i>\<t>\<i>\<o>\<n> C \<Longrightarrow> (\<c>\<o>\<n>\<d>\<i>\<t>\<i>\<o>\<n> False) \<or>\<^sub>c\<^sub>u\<^sub>t (X \<t>\<r>\<a>\<n>\<s>\<f>\<o>\<r>\<m>\<s> A \<r>\<e>\<m>\<a>\<i>\<n>\<s> R \<w>\<i>\<t>\<h> P))
+\<Longrightarrow> (\<c>\<o>\<n>\<d>\<i>\<t>\<i>\<o>\<n> \<not> C \<Longrightarrow> (\<c>\<o>\<n>\<d>\<i>\<t>\<i>\<o>\<n> False) \<or>\<^sub>c\<^sub>u\<^sub>t (X \<t>\<r>\<a>\<n>\<s>\<f>\<o>\<r>\<m>\<s> B \<r>\<e>\<m>\<a>\<i>\<n>\<s> R \<w>\<i>\<t>\<h> P))
+\<Longrightarrow> X \<t>\<r>\<a>\<n>\<s>\<f>\<o>\<r>\<m>\<s> (if C then A else B) \<r>\<e>\<m>\<a>\<i>\<n>\<s> R \<w>\<i>\<t>\<h> P \<close>
+  by (cases C; simp add: Premise_def)
+
 
 
 subsection \<open>Top\<close>
 
-lemma [\<phi>reason 2550]:
+lemma [\<phi>reason 2600]:
   \<open>Any \<t>\<r>\<a>\<n>\<s>\<f>\<o>\<r>\<m>\<s> \<top>\<close>
   unfolding Transformation_def by blast
 
 (*The following procedure only considers commutative semigroup*)
 
-lemma [\<phi>reason 2555 if \<open>fn (ctxt,sequent) =>
+lemma [\<phi>reason 2605 if \<open>fn (ctxt,sequent) =>
           case Thm.major_prem_of sequent
             of _ (*Trueprop*) $ (_ (*transformation*) $ _ $ (_ (*times*) $ R $ _) $ _)
                => let fun chk (Const(\<^const_name>\<open>times\<close>, _) $ X $ Const(\<^const_name>\<open>top\<close>, _)) = chk X
@@ -905,15 +946,22 @@ lemma [\<phi>reason 2555 if \<open>fn (ctxt,sequent) =>
   until the last one which can be done by \<open>Any \<t>\<r>\<a>\<n>\<s>\<f>\<o>\<r>\<m>\<s> \<top>\<close> directly.
   Again we assume and only consider commutative semigroup*)
 
-lemma [\<phi>reason 2550]:
+lemma [\<phi>reason 2600]:
   \<open> A \<t>\<r>\<a>\<n>\<s>\<f>\<o>\<r>\<m>\<s> R \<w>\<i>\<t>\<h> P
 \<Longrightarrow> A * B \<t>\<r>\<a>\<n>\<s>\<f>\<o>\<r>\<m>\<s> R * \<top> \<w>\<i>\<t>\<h> P\<close>
   for A :: \<open>'a::sep_ab_semigroup BI\<close>
   unfolding Transformation_def
   by clarsimp blast
 
+lemma [\<phi>reason 2595]:
+  \<open> A \<t>\<r>\<a>\<n>\<s>\<f>\<o>\<r>\<m>\<s> R \<w>\<i>\<t>\<h> P
+\<Longrightarrow> A \<t>\<r>\<a>\<n>\<s>\<f>\<o>\<r>\<m>\<s> R * \<top> \<w>\<i>\<t>\<h> P\<close>
+  for A :: \<open>'a::sep_algebra BI\<close>
+  unfolding Transformation_def
+  by clarsimp (metis mult_1_class.mult_1_right sep_magma_1_left)
+
 lemma [\<phi>reason 0]:
-  \<open> FAIL TEXT(\<open>Sorry, currently we cannot solve \<open>R * \<top>\<close> problems on non-commutative group.\<close>)
+  \<open> FAIL TEXT(\<open>Sorry, currently we do not support solving \<open>R * \<top>\<close> problems on non-monoidal-commutative group.\<close>)
 \<Longrightarrow> X \<t>\<r>\<a>\<n>\<s>\<f>\<o>\<r>\<m>\<s> R * \<top> \<w>\<i>\<t>\<h> P\<close>
   unfolding Transformation_def
   by blast
@@ -1068,10 +1116,10 @@ lemma [\<phi>reason 60 for \<open> _ * _ \<t>\<r>\<a>\<n>\<s>\<f>\<o>\<r>\<m>\<s
 *)  
 
 (* lemma [\<phi>reason 1200
-    on \<open>?R \<t>\<r>\<a>\<n>\<s>\<f>\<o>\<r>\<m>\<s> ?R' \<heavy_comma> \<blangle> OBJ ?a \<Zinj> ?x \<Ztypecolon> ?X \<brangle> \<w>\<i>\<t>\<h> ?P \<^bold>d\<^bold>u\<^bold>a\<^bold>l ?R'\<^sub>m \<heavy_comma> VAL ?V \<heavy_comma> \<blangle> OBJ ?a\<^sub>m \<Zinj> ?x\<^sub>m \<Ztypecolon> ?X\<^sub>m \<brangle> \<longmapsto> ?R\<^sub>m \<^bold>@\<^bold>G\<^bold>O\<^bold>A\<^bold>L ?G\<close>
+    on \<open>?R \<t>\<r>\<a>\<n>\<s>\<f>\<o>\<r>\<m>\<s> ?R' \<heavy_comma> \<blangle> OBJ ?a \<Zinj> ?x \<Ztypecolon> ?X \<brangle> \<w>\<i>\<t>\<h> ?P \<^bold>d\<^bold>u\<^bold>a\<^bold>l ?R'\<^sub>m \<heavy_comma> VAL ?V \<heavy_comma> \<blangle> OBJ ?a\<^sub>m \<Zinj> ?x\<^sub>m \<Ztypecolon> ?X\<^sub>m \<brangle> \<longmapsto> ?R\<^sub>m @GOAL ?G\<close>
   ]: \<comment> \<open>OR search the later cells, if hasn't succeeded.\<close>
-  " R \<t>\<r>\<a>\<n>\<s>\<f>\<o>\<r>\<m>\<s> R' \<heavy_comma> \<blangle> OBJ a \<Zinj> x \<Ztypecolon> X \<brangle> \<w>\<i>\<t>\<h> P \<^bold>d\<^bold>u\<^bold>a\<^bold>l R'\<^sub>m \<heavy_comma> \<blangle> OBJ a\<^sub>m \<Zinj> x\<^sub>m \<Ztypecolon> X\<^sub>m \<brangle> \<longmapsto> R\<^sub>m \<^bold>@\<^bold>G\<^bold>O\<^bold>A\<^bold>L G
-\<Longrightarrow> R \<t>\<r>\<a>\<n>\<s>\<f>\<o>\<r>\<m>\<s> R' \<heavy_comma> \<blangle> OBJ a \<Zinj> x \<Ztypecolon> X \<brangle> \<w>\<i>\<t>\<h> P \<^bold>d\<^bold>u\<^bold>a\<^bold>l R'\<^sub>m \<heavy_comma> VAL V \<heavy_comma> \<blangle> OBJ a\<^sub>m \<Zinj> x\<^sub>m \<Ztypecolon> X\<^sub>m \<brangle> \<longmapsto> R\<^sub>m \<heavy_comma> VAL V \<^bold>@\<^bold>G\<^bold>O\<^bold>A\<^bold>L G"
+  " R \<t>\<r>\<a>\<n>\<s>\<f>\<o>\<r>\<m>\<s> R' \<heavy_comma> \<blangle> OBJ a \<Zinj> x \<Ztypecolon> X \<brangle> \<w>\<i>\<t>\<h> P \<^bold>d\<^bold>u\<^bold>a\<^bold>l R'\<^sub>m \<heavy_comma> \<blangle> OBJ a\<^sub>m \<Zinj> x\<^sub>m \<Ztypecolon> X\<^sub>m \<brangle> \<longmapsto> R\<^sub>m @GOAL G
+\<Longrightarrow> R \<t>\<r>\<a>\<n>\<s>\<f>\<o>\<r>\<m>\<s> R' \<heavy_comma> \<blangle> OBJ a \<Zinj> x \<Ztypecolon> X \<brangle> \<w>\<i>\<t>\<h> P \<^bold>d\<^bold>u\<^bold>a\<^bold>l R'\<^sub>m \<heavy_comma> VAL V \<heavy_comma> \<blangle> OBJ a\<^sub>m \<Zinj> x\<^sub>m \<Ztypecolon> X\<^sub>m \<brangle> \<longmapsto> R\<^sub>m \<heavy_comma> VAL V @GOAL G"
   unfolding FOCUS_TAG_def Subty_Target2_def Separation_assoc[symmetric]
     Separation_comm(2)[of "VAL V" "\<tort_lbrace>a\<^sub>m \<Zinj> x\<^sub>m \<Ztypecolon> X\<^sub>m\<tort_rbrace>"]
   unfolding Separation_assoc
